fsub/autosubst2_dctx/prop_subtyping.v
@@ -1,0 +1,20 @@
+Require Import common.prop_as_core.
+Require Import common.prop_as_unscoped.
+Require Import fsub.autosubst2_dctx.def_as2.
+Require Import fsub.autosubst2_dctx.def_extra.
+
+From Coq Require Import ssreflect ssrfun ssrbool.
+From Hammer Require Import Tactics.
+Require Import Coq.Program.Equality.
+Require Import List.
+
+Import SubstNotations.
+Import UnscopedNotations.
+
+Theorem subtyping_reflexivity Δ A : 
+  Δ ⊢ A ->
+  Δ ⊢ A <: A.
+Proof.
+  move : Δ; elim: A; intros; try hauto ctrs:subtyping.
+  apply sub_top; eauto.
+Qed.
